code/libs/list-modulo-permutation/olist.v
@@ -1,0 +1,20 @@
+From Stdlib Require Export Sets.Multiset.
+From Stdlib Require Export List.
+Export ListNotations.
+
+Module lists_abella.
+
+(** TODO: olist is a list of "o's" *)
+
+Definition o := nat.
+
+Inductive append : list o -> list o -> list o -> Prop :=
+  | append_nil (L : list o): append [] L L
+  | append_cons e J K L: append (e :: J) K (e :: L).
+
+Inductive rev : list o -> list o -> Prop :=
+| rev_nil : rev [] []
+| rev_cons e J L (H : exists K, rev J K /\ append K (e :: []) L ) : rev J L.
+
+
+End lists_abella.
